Weidenbach_Book/Array_UInt.thy
@@ -1377,5 +1377,184 @@ lemma delete_index_and_swap_aa_i32_u64_ll_hnr_u[sepref_fr_rules]:
   by sepref_to_hoare (sep_auto dest: le_length_ll_nemptyD
       simp: delete_index_and_swap_ll_def update_ll_def last_ll_def set_butlast_ll_def
       length_ll_def[symmetric] uint32_nat_rel_def br_def uint64_nat_rel_def)
+
+definition swap_aa_i32_u64  :: "('a::{heap,default}) arrayO_raa \<Rightarrow> uint32 \<Rightarrow> uint64 \<Rightarrow> uint64 \<Rightarrow> 'a arrayO_raa Heap" where
+  \<open>swap_aa_i32_u64 xs k i j = do {
+    xi \<leftarrow> arl_get_u xs k;
+    xj \<leftarrow> swap_u64_code xi i j;
+    xs \<leftarrow> arl_set_u xs k xj;
+    return xs
+  }\<close>
+lemma arrayO_arl_get_u_rule[sep_heap_rules]:
+  assumes i: \<open>i < length a\<close> and \<open>(i' , i) \<in> uint32_nat_rel\<close>
+  shows \<open><arlO_assn (array_assn R) a ai> arl_get_u ai i' <\<lambda>r. arlO_assn_except (array_assn R) [i] a ai
+   (\<lambda>r'. array_assn R (a ! i) r * \<up>(r = r' ! i))>\<close>
+  using assms
+  by (sep_auto simp: arl_get_u_def arl_get'_def nat_of_uint32_code[symmetric]
+      uint32_nat_rel_def br_def)
+
+lemma swap_aa_i32_u64_hnr[sepref_fr_rules]:
+  assumes \<open>is_pure R\<close>
+  shows \<open>(uncurry3 swap_aa_i32_u64, uncurry3 (RETURN oooo swap_ll)) \<in>
+   [\<lambda>(((xs, k), i), j). k < length xs \<and> i < length_rll xs k \<and> j < length_rll xs k]\<^sub>a
+  (arlO_assn (array_assn R))\<^sup>d *\<^sub>a uint32_nat_assn\<^sup>k *\<^sub>a uint64_nat_assn\<^sup>k *\<^sub>a uint64_nat_assn\<^sup>k \<rightarrow>
+    (arlO_assn (array_assn R))\<close>
+proof -
+  note update_raa_rule_pure[sep_heap_rules]
+  obtain R' where R': \<open>R' = the_pure R\<close> and RR': \<open>R = pure R'\<close>
+    using assms by fastforce
+  have [simp]: \<open>the_pure (\<lambda>a b. \<up> ((b, a) \<in> R')) = R'\<close>
+    unfolding pure_def[symmetric] by auto
+  have H: \<open><is_array_list p (aa, bc) *
+       heap_list_all_nth (array_assn (\<lambda>a c. \<up> ((c, a) \<in> R'))) (remove1 bb [0..<length p]) a p *
+       array_assn (\<lambda>a c. \<up> ((c, a) \<in> R')) (a ! bb) (p ! bb)>
+      Array.nth (p ! bb) (nat_of_integer (integer_of_uint64 bia))
+      <\<lambda>r. \<exists>\<^sub>A p'. is_array_list p' (aa, bc) * \<up> (bb < length p' \<and> p' ! bb = p ! bb \<and> length a = length p') *
+          heap_list_all_nth (array_assn (\<lambda>a c. \<up> ((c, a) \<in> R'))) (remove1 bb [0..<length p']) a p' *
+         array_assn (\<lambda>a c. \<up> ((c, a) \<in> R')) (a ! bb) (p' ! bb) *
+         R (a ! bb ! (nat_of_uint64 bia)) r >\<close>
+    if
+      \<open>is_pure (\<lambda>a c. \<up> ((c, a) \<in> R'))\<close> and
+      \<open>bb < length p\<close> and
+      \<open>nat_of_uint64 bia < length (a ! bb)\<close> and
+      \<open>nat_of_uint64 bi < length (a ! bb)\<close> and
+      \<open>length a = length p\<close>
+    for bi :: \<open>uint64\<close> and bia :: \<open>uint64\<close> and bb :: \<open>nat\<close> and a :: \<open>'a list list\<close> and
+      aa :: \<open>'b array array\<close> and bc :: \<open>nat\<close> and p :: \<open>'b array list\<close>
+    using that
+    by (sep_auto simp: array_assn_def hr_comp_def is_array_def nat_of_uint64_code[symmetric]
+        list_rel_imp_same_length RR' pure_def param_nth)
+  have H': \<open>is_array_list p' (aa, ba) * p' ! bb \<mapsto>\<^sub>a b [nat_of_uint64 bia := b ! nat_of_uint64 bi,
+             nat_of_uint64 bi := xa] *
+      heap_list_all_nth (\<lambda>a b.  \<exists>\<^sub>Aba.  b \<mapsto>\<^sub>a ba *  \<up> ((ba, a) \<in> \<langle>R'\<rangle>list_rel))
+          (remove1 bb [0..<length p']) a p' * R (a ! bb ! nat_of_uint64 bia) xa \<Longrightarrow>\<^sub>A
+      is_array_list p' (aa, ba) *
+      heap_list_all
+       (\<lambda>a c. \<exists>\<^sub>Ab. c \<mapsto>\<^sub>a b *  \<up> ((b, a) \<in> \<langle>R'\<rangle>list_rel))
+       (a[bb := (a ! bb) [nat_of_uint64 bia := a ! bb ! nat_of_uint64 bi,
+             nat_of_uint64 bi := a ! bb ! nat_of_uint64 bia]])
+        p' *  true\<close>
+    if
+      \<open>is_pure (\<lambda>a c. \<up> ((c, a) \<in> R'))\<close> and
+      le: \<open>nat_of_uint64 bia < length (a ! bb)\<close> and
+      le': \<open>nat_of_uint64 bi < length (a ! bb)\<close> and
+      \<open>bb < length p'\<close> and
+      \<open>length a = length p'\<close> and
+      a: \<open>(b, a ! bb) \<in> \<langle>R'\<rangle>list_rel\<close>
+    for bi :: \<open>uint64\<close> and bia :: \<open>uint64\<close> and bb :: \<open>nat\<close> and a :: \<open>'a list list\<close> and
+      xa :: \<open>'b\<close> and p' :: \<open>'b array list\<close> and b :: \<open>'b list\<close> and aa :: \<open>'b array array\<close> and ba :: \<open>nat\<close>
+  proof -
+    have 1: \<open>(b[nat_of_uint64 bia := b ! nat_of_uint64 bi, nat_of_uint64 bi := xa],
+   (a ! bb)[nat_of_uint64 bia := a ! bb ! nat_of_uint64 bi,
+   nat_of_uint64 bi := a ! bb ! nat_of_uint64 bia]) \<in> \<langle>R'\<rangle>list_rel\<close>
+      if \<open>(xa, a ! bb ! nat_of_uint64 bia) \<in> R'\<close>
+      using that a le le'
+      unfolding list_rel_def list_all2_conv_all_nth
+      by auto
+    have 2: \<open>heap_list_all_nth (\<lambda>a b. \<exists>\<^sub>Aba. b \<mapsto>\<^sub>a ba * \<up> ((ba, a) \<in> \<langle>R'\<rangle>list_rel)) (remove1 bb [0..<length p']) a p' =
+    heap_list_all_nth (\<lambda>a c. \<exists>\<^sub>Ab. c \<mapsto>\<^sub>a b * \<up> ((b, a) \<in> \<langle>R'\<rangle>list_rel)) (remove1 bb [0..<length p'])
+     (a[bb := (a ! bb)[nat_of_uint64 bia := a ! bb ! nat_of_uint64 bi, nat_of_uint64 bi := a ! bb ! nat_of_uint64 bia]]) p'\<close>
+      by (rule heap_list_all_nth_cong)  auto
+    show ?thesis using that
+      unfolding heap_list_all_heap_list_all_nth_eq
+      by (subst (2) heap_list_all_nth_remove1[of bb])
+        (sep_auto simp:  heap_list_all_heap_list_all_nth_eq swap_def fr_refl RR'
+          pure_def 2[symmetric] intro!: 1)+
+  qed
+
+  show ?thesis
+    using assms unfolding R'[symmetric] unfolding RR'
+    apply sepref_to_hoare
+
+    apply (sep_auto simp: swap_aa_i32_u64_def swap_ll_def arlO_assn_except_def length_rll_def
+        length_rll_update_rll nth_raa_i_u64_def uint64_nat_rel_def br_def
+        swap_def nth_rll_def list_update_swap swap_u64_code_def nth_u64_code_def Array.nth'_def
+        heap_array_set_u64_def heap_array_set'_u64_def arl_assn_def
+         Array.upd'_def)
+    apply (rule H; assumption)
+    apply (sep_auto simp: array_assn_def nat_of_uint64_code[symmetric] hr_comp_def is_array_def
+        list_rel_imp_same_length arlO_assn_def arl_assn_def hr_comp_def[abs_def] arl_set_u_def
+        arl_set'_u_def list_rel_pres_length uint32_nat_rel_def br_def)
+    apply (rule H'; assumption)
+    done
+qed
+
+
+
+definition length_raa_i32_u :: \<open>'a::heap arrayO_raa \<Rightarrow> uint32 \<Rightarrow> uint32 Heap\<close> where
+  \<open>length_raa_i32_u xs i = do {
+     x \<leftarrow> arl_get_u xs i;
+    length_u_code x}\<close>
+
+lemma length_raa_i32_rule[sep_heap_rules]:
+  assumes \<open>nat_of_uint32 b < length xs\<close>
+  shows \<open><arlO_assn (array_assn R) xs a> length_raa_i32_u a b
+   <\<lambda>r. arlO_assn (array_assn R) xs a * \<up> (r = uint32_of_nat (length_rll xs (nat_of_uint32 b)))>\<^sub>t\<close>
+proof -
+  have 1: \<open>a * b* c = c * a *b\<close> for a b c :: assn
+    by (auto simp: ac_simps)
+  have [sep_heap_rules]: \<open><arlO_assn_except (array_assn R) [nat_of_uint32 b] xs a
+           (\<lambda>r'. array_assn R (xs ! nat_of_uint32 b) x *
+                 \<up> (x = r' ! nat_of_uint32 b))>
+         Array.len x <\<lambda>r.  arlO_assn (array_assn R) xs a *
+                 \<up> (r = length (xs ! nat_of_uint32 b))>\<close>
+    for x
+    unfolding arlO_assn_except_def
+    apply (subst arlO_assn_except_array0_index[symmetric, OF assms])
+    apply sep_auto
+    apply (subst 1)
+    by (sep_auto simp: array_assn_def is_array_def hr_comp_def list_rel_imp_same_length
+        arlO_assn_except_def)
+  show ?thesis
+    using assms
+    unfolding length_raa_i32_u_def length_u_code_def arl_get_u_def arl_get'_def length_rll_def
+    by (sep_auto simp: nat_of_uint32_code[symmetric])
+qed
+
+lemma length_raa_i32_u_hnr[sepref_fr_rules]:
+  shows \<open>(uncurry length_raa_i32_u, uncurry (RETURN \<circ>\<circ> length_rll_n_uint32)) \<in>
+     [\<lambda>(xs, i). i < length xs \<and> length (xs ! i) \<le> uint32_max]\<^sub>a
+       (arlO_assn (array_assn R))\<^sup>k *\<^sub>a uint32_nat_assn\<^sup>k \<rightarrow> uint32_nat_assn\<close>
+  by sepref_to_hoare (sep_auto simp: uint32_nat_rel_def br_def length_rll_def
+      nat_of_uint32_uint32_of_nat_id)+
+
+definition (in -)length_aa_u64_o64 :: \<open>('a::heap array_list) array \<Rightarrow> uint64 \<Rightarrow> uint64 Heap\<close> where
+  \<open>length_aa_u64_o64 xs i = length_aa_u64 xs i >>= (\<lambda>n. return (uint64_of_nat n))\<close>
+
+definition arl_length_o64 where
+  \<open>arl_length_o64 x = do {n \<leftarrow> arl_length x;  return (uint64_of_nat n)}\<close>
+
+lemma length_aa_u64_o64_code[code]:
+  \<open>length_aa_u64_o64 xs i = nth_u64_code xs i \<bind> arl_length_o64\<close>
+  unfolding length_aa_u64_o64_def length_aa_u64_def nth_u_def[symmetric] nth_u64_code_def
+   Array.nth'_def arl_length_o64_def length_aa_def
+  by (auto simp: nat_of_uint32_code nat_of_uint64_code[symmetric])
+
+lemma length_aa_u64_o64_hnr[sepref_fr_rules]:
+   \<open>(uncurry length_aa_u64_o64, uncurry (RETURN \<circ>\<circ> length_ll)) \<in>
+     [\<lambda>(xs, i). i < length xs \<and> length (xs ! i) \<le> uint64_max]\<^sub>a
+    (arrayO_assn (arl_assn R))\<^sup>k *\<^sub>a uint64_nat_assn\<^sup>k \<rightarrow> uint64_nat_assn\<close>
+  by sepref_to_hoare (sep_auto simp: uint32_nat_rel_def length_aa_u64_o64_def br_def
+     length_aa_u64_def uint64_nat_rel_def nat_of_uint64_uint64_of_nat_id
+     length_ll_def)
+
+
+definition (in -)length_aa_u32_o64 :: \<open>('a::heap array_list) array \<Rightarrow> uint32 \<Rightarrow> uint64 Heap\<close> where
+  \<open>length_aa_u32_o64 xs i = length_aa_u xs i >>= (\<lambda>n. return (uint64_of_nat n))\<close>
+
+lemma length_aa_u32_o64_code[code]:
+  \<open>length_aa_u32_o64 xs i = nth_u_code xs i \<bind> arl_length_o64\<close>
+  unfolding length_aa_u32_o64_def length_aa_u64_def nth_u_def[symmetric] nth_u_code_def
+   Array.nth'_def arl_length_o64_def length_aa_u_def length_aa_def
+  by (auto simp: nat_of_uint64_code[symmetric] nat_of_uint32_code[symmetric])
+
+lemma length_aa_u32_o64_hnr[sepref_fr_rules]:
+   \<open>(uncurry length_aa_u32_o64, uncurry (RETURN \<circ>\<circ> length_ll)) \<in>
+     [\<lambda>(xs, i). i < length xs \<and> length (xs ! i) \<le> uint64_max]\<^sub>a
+    (arrayO_assn (arl_assn R))\<^sup>k *\<^sub>a uint32_nat_assn\<^sup>k \<rightarrow> uint64_nat_assn\<close>
+  by sepref_to_hoare (sep_auto simp: uint32_nat_rel_def length_aa_u32_o64_def br_def
+     length_aa_u64_def uint64_nat_rel_def nat_of_uint64_uint64_of_nat_id
+     length_ll_def length_aa_u_def)
+
 (* End sort *)
 end
