Weidenbach_Book/IsaSAT_Clauses.thy
@@ -783,6 +783,23 @@ definition get_fresh_index_packed :: \<open>'v clauses_l \<Rightarrow> nat nres\
 \<open>get_fresh_index_packed N = SPEC(\<lambda>i. i > 0 \<and> i \<notin># dom_m N \<and>
     (\<forall>j < i. j > 0 \<longrightarrow> j \<in># dom_m N))\<close>
 
+lemma (in -)get_fresh_index_packed_alt_def: 
+  assumes \<open>packed N\<close>
+  shows \<open>get_fresh_index_packed N = SPEC (\<lambda>i. i = Suc (Max_dom N))\<close>
+proof -
+  have [iff]: \<open>j \<in># dom_m N \<longleftrightarrow> j > 0 \<and> j \<le> Max_dom N\<close> for j
+    using assms in_multiset_ge_Max[of j \<open>dom_m N\<close>]
+    unfolding packed_def
+    by (auto simp: get_fresh_index_packed_def packed_def
+        split: if_splits)
+  have \<open> \<forall>j<x. 0 < j \<longrightarrow> j \<le> Max_dom N \<Longrightarrow>
+         \<not> x \<le> Max_dom N \<Longrightarrow> x = Suc (Max_dom N)\<close> for x
+    by (cases \<open>x > Suc (Max_dom N)\<close>)  auto
+  then show ?thesis
+    by (auto simp: get_fresh_index_packed_def split: if_splits
+      dest: multi_member_split in_multiset_ge_Max)
+qed
+
 definition fm_add_new_packed where
  \<open>fm_add_new_packed b C N = do {
     i \<leftarrow> get_fresh_index_packed N;
@@ -989,111 +1006,6 @@ proof -
     using pre ..
 qed
 
-definition swap_aa_i32_u64  :: "('a::{heap,default}) arrayO_raa \<Rightarrow> uint32 \<Rightarrow> uint64 \<Rightarrow> uint64 \<Rightarrow> 'a arrayO_raa Heap" where
-  \<open>swap_aa_i32_u64 xs k i j = do {
-    xi \<leftarrow> arl_get_u xs k;
-    xj \<leftarrow> swap_u64_code xi i j;
-    xs \<leftarrow> arl_set_u xs k xj;
-    return xs
-  }\<close>
-
-(* TODO Move and adapt proofs *)
-lemma arrayO_arl_get_u_rule[sep_heap_rules]:
-  assumes i: \<open>i < length a\<close> and \<open>(i' , i) \<in> uint32_nat_rel\<close>
-  shows \<open><arlO_assn (array_assn R) a ai> arl_get_u ai i' <\<lambda>r. arlO_assn_except (array_assn R) [i] a ai
-   (\<lambda>r'. array_assn R (a ! i) r * \<up>(r = r' ! i))>\<close>
-  using assms
-  by (sep_auto simp: arl_get_u_def arl_get'_def nat_of_uint32_code[symmetric]
-      uint32_nat_rel_def br_def)
-(* END Move *)
-
-lemma swap_aa_i32_u64_hnr[sepref_fr_rules]:
-  assumes \<open>is_pure R\<close>
-  shows \<open>(uncurry3 swap_aa_i32_u64, uncurry3 (RETURN oooo swap_ll)) \<in>
-   [\<lambda>(((xs, k), i), j). k < length xs \<and> i < length_rll xs k \<and> j < length_rll xs k]\<^sub>a
-  (arlO_assn (array_assn R))\<^sup>d *\<^sub>a uint32_nat_assn\<^sup>k *\<^sub>a uint64_nat_assn\<^sup>k *\<^sub>a uint64_nat_assn\<^sup>k \<rightarrow>
-    (arlO_assn (array_assn R))\<close>
-proof -
-  note update_raa_rule_pure[sep_heap_rules]
-  obtain R' where R': \<open>R' = the_pure R\<close> and RR': \<open>R = pure R'\<close>
-    using assms by fastforce
-  have [simp]: \<open>the_pure (\<lambda>a b. \<up> ((b, a) \<in> R')) = R'\<close>
-    unfolding pure_def[symmetric] by auto
-  have H: \<open><is_array_list p (aa, bc) *
-       heap_list_all_nth (array_assn (\<lambda>a c. \<up> ((c, a) \<in> R'))) (remove1 bb [0..<length p]) a p *
-       array_assn (\<lambda>a c. \<up> ((c, a) \<in> R')) (a ! bb) (p ! bb)>
-      Array.nth (p ! bb) (nat_of_integer (integer_of_uint64 bia))
-      <\<lambda>r. \<exists>\<^sub>A p'. is_array_list p' (aa, bc) * \<up> (bb < length p' \<and> p' ! bb = p ! bb \<and> length a = length p') *
-          heap_list_all_nth (array_assn (\<lambda>a c. \<up> ((c, a) \<in> R'))) (remove1 bb [0..<length p']) a p' *
-         array_assn (\<lambda>a c. \<up> ((c, a) \<in> R')) (a ! bb) (p' ! bb) *
-         R (a ! bb ! (nat_of_uint64 bia)) r >\<close>
-    if
-      \<open>is_pure (\<lambda>a c. \<up> ((c, a) \<in> R'))\<close> and
-      \<open>bb < length p\<close> and
-      \<open>nat_of_uint64 bia < length (a ! bb)\<close> and
-      \<open>nat_of_uint64 bi < length (a ! bb)\<close> and
-      \<open>length a = length p\<close>
-    for bi :: \<open>uint64\<close> and bia :: \<open>uint64\<close> and bb :: \<open>nat\<close> and a :: \<open>'a list list\<close> and
-      aa :: \<open>'b array array\<close> and bc :: \<open>nat\<close> and p :: \<open>'b array list\<close>
-    using that
-    by (sep_auto simp: array_assn_def hr_comp_def is_array_def nat_of_uint64_code[symmetric]
-        list_rel_imp_same_length RR' pure_def param_nth)
-  have H': \<open>is_array_list p' (aa, ba) * p' ! bb \<mapsto>\<^sub>a b [nat_of_uint64 bia := b ! nat_of_uint64 bi,
-             nat_of_uint64 bi := xa] *
-      heap_list_all_nth (\<lambda>a b.  \<exists>\<^sub>Aba.  b \<mapsto>\<^sub>a ba *  \<up> ((ba, a) \<in> \<langle>R'\<rangle>list_rel))
-          (remove1 bb [0..<length p']) a p' * R (a ! bb ! nat_of_uint64 bia) xa \<Longrightarrow>\<^sub>A
-      is_array_list p' (aa, ba) *
-      heap_list_all
-       (\<lambda>a c. \<exists>\<^sub>Ab. c \<mapsto>\<^sub>a b *  \<up> ((b, a) \<in> \<langle>R'\<rangle>list_rel))
-       (a[bb := (a ! bb) [nat_of_uint64 bia := a ! bb ! nat_of_uint64 bi,
-             nat_of_uint64 bi := a ! bb ! nat_of_uint64 bia]])
-        p' *  true\<close>
-    if
-      \<open>is_pure (\<lambda>a c. \<up> ((c, a) \<in> R'))\<close> and
-      le: \<open>nat_of_uint64 bia < length (a ! bb)\<close> and
-      le': \<open>nat_of_uint64 bi < length (a ! bb)\<close> and
-      \<open>bb < length p'\<close> and
-      \<open>length a = length p'\<close> and
-      a: \<open>(b, a ! bb) \<in> \<langle>R'\<rangle>list_rel\<close>
-    for bi :: \<open>uint64\<close> and bia :: \<open>uint64\<close> and bb :: \<open>nat\<close> and a :: \<open>'a list list\<close> and
-      xa :: \<open>'b\<close> and p' :: \<open>'b array list\<close> and b :: \<open>'b list\<close> and aa :: \<open>'b array array\<close> and ba :: \<open>nat\<close>
-  proof -
-    have 1: \<open>(b[nat_of_uint64 bia := b ! nat_of_uint64 bi, nat_of_uint64 bi := xa],
-   (a ! bb)[nat_of_uint64 bia := a ! bb ! nat_of_uint64 bi,
-   nat_of_uint64 bi := a ! bb ! nat_of_uint64 bia]) \<in> \<langle>R'\<rangle>list_rel\<close>
-      if \<open>(xa, a ! bb ! nat_of_uint64 bia) \<in> R'\<close>
-      using that a le le'
-      unfolding list_rel_def list_all2_conv_all_nth
-      by auto
-    have 2: \<open>heap_list_all_nth (\<lambda>a b. \<exists>\<^sub>Aba. b \<mapsto>\<^sub>a ba * \<up> ((ba, a) \<in> \<langle>R'\<rangle>list_rel)) (remove1 bb [0..<length p']) a p' =
-    heap_list_all_nth (\<lambda>a c. \<exists>\<^sub>Ab. c \<mapsto>\<^sub>a b * \<up> ((b, a) \<in> \<langle>R'\<rangle>list_rel)) (remove1 bb [0..<length p'])
-     (a[bb := (a ! bb)[nat_of_uint64 bia := a ! bb ! nat_of_uint64 bi, nat_of_uint64 bi := a ! bb ! nat_of_uint64 bia]]) p'\<close>
-      by (rule heap_list_all_nth_cong)  auto
-    show ?thesis using that
-      unfolding heap_list_all_heap_list_all_nth_eq
-      by (subst (2) heap_list_all_nth_remove1[of bb])
-        (sep_auto simp:  heap_list_all_heap_list_all_nth_eq swap_def fr_refl RR'
-          pure_def 2[symmetric] intro!: 1)+
-  qed
-
-  show ?thesis
-    using assms unfolding R'[symmetric] unfolding RR'
-    apply sepref_to_hoare
-
-    apply (sep_auto simp: swap_aa_i32_u64_def swap_ll_def arlO_assn_except_def length_rll_def
-        length_rll_update_rll nth_raa_i_u64_def uint64_nat_rel_def br_def
-        swap_def nth_rll_def list_update_swap swap_u64_code_def nth_u64_code_def Array.nth'_def
-        heap_array_set_u64_def heap_array_set'_u64_def arl_assn_def
-         Array.upd'_def)
-    apply (rule H; assumption)
-    apply (sep_auto simp: array_assn_def nat_of_uint64_code[symmetric] hr_comp_def is_array_def
-        list_rel_imp_same_length arlO_assn_def arl_assn_def hr_comp_def[abs_def] arl_set_u_def
-        arl_set'_u_def list_rel_pres_length uint32_nat_rel_def br_def)
-    apply (rule H'; assumption)
-    done
-qed
-
-
 sepref_definition fmap_swap_ll_i32_u64_clss
   is \<open>uncurry3 (RETURN oooo (\<lambda>(N, xs) i j k. (swap_ll N i j k, xs)))\<close>
   ::\<open>[\<lambda>((((xs, _), k), i), j). k < length xs \<and> i < length_rll xs k \<and> j < length_rll xs k]\<^sub>a
@@ -1249,44 +1161,6 @@ proof -
     using H unfolding f im apply assumption
     using pre ..
 qed
-
-
-definition length_raa_i32_u :: \<open>'a::heap arrayO_raa \<Rightarrow> uint32 \<Rightarrow> uint32 Heap\<close> where
-  \<open>length_raa_i32_u xs i = do {
-     x \<leftarrow> arl_get_u xs i;
-    length_u_code x}\<close>
-
-lemma length_raa_i32_rule[sep_heap_rules]:
-  assumes \<open>nat_of_uint32 b < length xs\<close>
-  shows \<open><arlO_assn (array_assn R) xs a> length_raa_i32_u a b
-   <\<lambda>r. arlO_assn (array_assn R) xs a * \<up> (r = uint32_of_nat (length_rll xs (nat_of_uint32 b)))>\<^sub>t\<close>
-proof -
-  have 1: \<open>a * b* c = c * a *b\<close> for a b c :: assn
-    by (auto simp: ac_simps)
-  have [sep_heap_rules]: \<open><arlO_assn_except (array_assn R) [nat_of_uint32 b] xs a
-           (\<lambda>r'. array_assn R (xs ! nat_of_uint32 b) x *
-                 \<up> (x = r' ! nat_of_uint32 b))>
-         Array.len x <\<lambda>r.  arlO_assn (array_assn R) xs a *
-                 \<up> (r = length (xs ! nat_of_uint32 b))>\<close>
-    for x
-    unfolding arlO_assn_except_def
-    apply (subst arlO_assn_except_array0_index[symmetric, OF assms])
-    apply sep_auto
-    apply (subst 1)
-    by (sep_auto simp: array_assn_def is_array_def hr_comp_def list_rel_imp_same_length
-        arlO_assn_except_def)
-  show ?thesis
-    using assms
-    unfolding length_raa_i32_u_def length_u_code_def arl_get_u_def arl_get'_def length_rll_def
-    by (sep_auto simp: nat_of_uint32_code[symmetric])
-qed
-
-lemma length_raa_i32_u_hnr[sepref_fr_rules]:
-  shows \<open>(uncurry length_raa_i32_u, uncurry (RETURN \<circ>\<circ> length_rll_n_uint32)) \<in>
-     [\<lambda>(xs, i). i < length xs \<and> length (xs ! i) \<le> uint32_max]\<^sub>a
-       (arlO_assn (array_assn R))\<^sup>k *\<^sub>a uint32_nat_assn\<^sup>k \<rightarrow> uint32_nat_assn\<close>
-  by sepref_to_hoare (sep_auto simp: uint32_nat_rel_def br_def length_rll_def
-      nat_of_uint32_uint32_of_nat_id)+
 
 sepref_definition fmap_length_rll_u32_clss
   is \<open>uncurry (RETURN oo (\<lambda>(N, _) i. length_rll_n_uint32 N i))\<close>
